@prefix : <http://www.kolitha.com/hcdt/> .
@prefix owl: <http://www.w3.org/2002/07/owl#> .
@prefix rdf: <http://www.w3.org/1999/02/22-rdf-syntax-ns#> .
@prefix xml: <http://www.w3.org/XML/1998/namespace> .
@prefix xsd: <http://www.w3.org/2001/XMLSchema#> .
@prefix rdfs: <http://www.w3.org/2000/01/rdf-schema#> .
@base <http://www.kolitha.com/hcdt/> .

<http://www.kolitha.com/hcdt> rdf:type owl:Ontology ;
                               owl:versionIRI <http://www.kolitha.com/hcdt> ;
                               rdfs:comment "A conceptual model for describing Human-Centered Digital Twin Characteristics, Functions and components" .

#################################################################
#    Annotation properties
#################################################################

###  http://ontologydesignpatterns.org/opla-sd#entityPosition
<http://ontologydesignpatterns.org/opla-sd#entityPosition> rdf:type owl:AnnotationProperty .


###  http://ontologydesignpatterns.org/opla-sd#entityPositionX
<http://ontologydesignpatterns.org/opla-sd#entityPositionX> rdf:type owl:AnnotationProperty .


###  http://ontologydesignpatterns.org/opla-sd#entityPositionY
<http://ontologydesignpatterns.org/opla-sd#entityPositionY> rdf:type owl:AnnotationProperty .


#################################################################
#    Object Properties
#################################################################

###  http://www.kolitha.com/hcdt/experiences
:experiences rdf:type owl:ObjectProperty ;
             rdfs:domain :HumanActor ;
             rdfs:range <http://www.sws.org/sws/HumanCentricityFactor> .


###  http://www.kolitha.com/hcdt/hasAction
:hasAction rdf:type owl:ObjectProperty ;
           rdfs:domain :DigitalTwinInstance ;
           rdfs:range :Action .


###  http://www.kolitha.com/hcdt/hasDigitalTwin
:hasDigitalTwin rdf:type owl:ObjectProperty ;
                rdfs:domain :HumanActor ;
                rdfs:range :HumanDigitalTwin .


###  http://www.kolitha.com/hcdt/hasLatency
:hasLatency rdf:type owl:ObjectProperty ;
            rdfs:domain :sosa:Sensor ;
            rdfs:range :ssn-system:Latency .


###  http://www.kolitha.com/hcdt/hasSkill
:hasSkill rdf:type owl:ObjectProperty ;
          rdfs:domain :Actor .


###  http://www.kolitha.com/hcdt/hasStatus
:hasStatus rdf:type owl:ObjectProperty ;
           rdfs:domain :Actor ;
           rdfs:range :Status .


###  http://www.kolitha.com/hcdt/hasVisualization
:hasVisualization rdf:type owl:ObjectProperty ;
                  rdfs:domain :Data ,
                              :DigitalTwinInstance ;
                  rdfs:range :Visualization .


###  http://www.kolitha.com/hcdt/interactsWith
:interactsWith rdf:type owl:ObjectProperty ;
               rdfs:domain :User ;
               rdfs:range :Interface .


###  http://www.kolitha.com/hcdt/isDisplayedOn
:isDisplayedOn rdf:type owl:ObjectProperty ;
               rdfs:domain :Visualization ;
               rdfs:range :Interface .


###  http://www.kolitha.com/hcdt/observesActor
:observesActor rdf:type owl:ObjectProperty ;
               rdfs:domain :sosa:Sensor ;
               rdfs:range :Actor .


###  http://www.kolitha.com/hcdt/observesHumanCentricityFactor
:observesHumanCentricityFactor rdf:type owl:ObjectProperty ;
                               rdfs:domain :sosa:Sensor ;
                               rdfs:range <http://www.sws.org/sws/HumanCentricityFactor> .


###  http://www.kolitha.com/hcdt/providesContextFor
:providesContextFor rdf:type owl:ObjectProperty ;
                    rdfs:domain :Context ;
                    rdfs:range :DigitalTwinInstance .


###  http://www.kolitha.com/hcdt/receiveData
:receiveData rdf:type owl:ObjectProperty ;
             owl:inverseOf :sendData ;
             rdfs:domain :Data ;
             rdfs:range :sosa:Sensor .


###  http://www.kolitha.com/hcdt/sendData
:sendData rdf:type owl:ObjectProperty ;
          rdfs:domain :sosa:Sensor ;
          rdfs:range :Data .


###  http://www.kolitha.com/hcdt/updateContext
:updateContext rdf:type owl:ObjectProperty ;
               rdfs:domain :Data ;
               rdfs:range :Context .


#################################################################
#    Data properties
#################################################################

###  http://www.kolitha.com/hcdt/hasLatencyValue
:hasLatencyValue rdf:type owl:DatatypeProperty .


###  http://www.kolitha.com/hcdt/hasStatusCode
:hasStatusCode rdf:type owl:DatatypeProperty .


###  http://www.kolitha.com/hcdt/hasTimestamp
:hasTimestamp rdf:type owl:DatatypeProperty .


###  http://www.kolitha.com/hcdt/hasUpdateFrequency
:hasUpdateFrequency rdf:type owl:DatatypeProperty .


#################################################################
#    Classes
#################################################################

###  http://www.kolitha.com/hcdt/Action
:Action rdf:type owl:Class ;
        rdfs:comment """Describes the intended use and operational behaviour of digital twins
through the functions or tasks they perform within the system.""" .


###  http://www.kolitha.com/hcdt/Actor
:Actor rdf:type owl:Class ;
       rdfs:comment "Represents an entity capable of performing tasks or making decisions." .


###  http://www.kolitha.com/hcdt/Context
:Context rdf:type owl:Class ;
         rdfs:comment "Any information that can be used to characterize the situation of an entity." .


###  http://www.kolitha.com/hcdt/ControlAction
:ControlAction rdf:type owl:Class ;
               rdfs:subClassOf :Action .


###  http://www.kolitha.com/hcdt/Data
:Data rdf:type owl:Class ;
      rdfs:comment "A collection of facts and statistics, including real-time and historical information, used for reference, analysis, and reasoning." .


###  http://www.kolitha.com/hcdt/DataVisualization
:DataVisualization rdf:type owl:Class ;
                   rdfs:subClassOf :Visualization .


###  http://www.kolitha.com/hcdt/DecisionAction
:DecisionAction rdf:type owl:Class ;
                rdfs:subClassOf :Action .


###  http://www.kolitha.com/hcdt/DerivedContext
:DerivedContext rdf:type owl:Class ;
                rdfs:subClassOf :Context ;
                rdfs:comment "Context inferred from raw data or calculated through processing, reasoning, or interpretations. (e.g., Workload)" .


###  http://www.kolitha.com/hcdt/DetectionAction
:DetectionAction rdf:type owl:Class ;
                 rdfs:subClassOf :Action .


###  http://www.kolitha.com/hcdt/DigitalModel
:DigitalModel rdf:type owl:Class ;
              rdfs:subClassOf :Visualization .


###  http://www.kolitha.com/hcdt/DigitalTwinInstance
:DigitalTwinInstance rdf:type owl:Class ;
                     rdfs:comment "Represents digital counterparts of real-world entities. Subclasses include HumanDigitalTwin, ProcessDigitalTwin, etc." .


###  http://www.kolitha.com/hcdt/HistoricalData
:HistoricalData rdf:type owl:Class ;
                rdfs:subClassOf :Data .


###  http://www.kolitha.com/hcdt/HumanActor
:HumanActor rdf:type owl:Class ;
            rdfs:subClassOf :Actor ;
            owl:disjointWith :NonHumanActor ;
            rdfs:comment "A subclass of Actor representing a human entity involved in performing tasks or making decisions" .


###  http://www.kolitha.com/hcdt/HumanDigitalTwin
:HumanDigitalTwin rdf:type owl:Class ;
                  rdfs:subClassOf :DigitalTwinInstance .


###  http://www.kolitha.com/hcdt/Interface
:Interface rdf:type owl:Class ;
           rdfs:comment "The point of interaction and communication" .


###  http://www.kolitha.com/hcdt/MonitoringAction
:MonitoringAction rdf:type owl:Class ;
                  rdfs:subClassOf :Action .


###  http://www.kolitha.com/hcdt/NonDerivedContext
:NonDerivedContext rdf:type owl:Class ;
                   rdfs:subClassOf :Context ;
                   rdfs:comment "Raw or directly observable contextual information (e.g., Temperature, Heart Rate)" .


###  http://www.kolitha.com/hcdt/NonHumanActor
:NonHumanActor rdf:type owl:Class ;
               rdfs:subClassOf :Actor ;
               rdfs:comment "A subclass of Actor representing artificial or automated entities, such as robots, AI or software, capable of performing tasks or making decisions." .


###  http://www.kolitha.com/hcdt/PredictionAction
:PredictionAction rdf:type owl:Class ;
                  rdfs:subClassOf :Action .


###  http://www.kolitha.com/hcdt/ProcessDigitalTwin
:ProcessDigitalTwin rdf:type owl:Class ;
                    rdfs:subClassOf :DigitalTwinInstance .


###  http://www.kolitha.com/hcdt/ProductDigitalTwin
:ProductDigitalTwin rdf:type owl:Class ;
                    rdfs:subClassOf :DigitalTwinInstance .


###  http://www.kolitha.com/hcdt/RealTimeData
:RealTimeData rdf:type owl:Class ;
              rdfs:subClassOf :Data .


###  http://www.kolitha.com/hcdt/Safety
:Safety rdf:type owl:Class ;
        rdfs:subClassOf <http://www.sws.org/sws/HumanCentricityFactor> .


###  http://www.kolitha.com/hcdt/Status
:Status rdf:type owl:Class ;
        rdfs:comment "Represents the operational state of an Actor." .


###  http://www.kolitha.com/hcdt/User
:User rdf:type owl:Class ;
      rdfs:comment "the User refers to the HumanActor who interacts with the system through an interface." .


###  http://www.kolitha.com/hcdt/Visualization
:Visualization rdf:type owl:Class ;
               rdfs:comment """The visual representation of Digital Twin instances and their associated
data""" .


###  http://www.kolitha.com/hcdt/esco:Skill
:esco:Skill rdf:type owl:Class ;
            rdfs:comment "A capability or competence possessed by an actor" .


###  http://www.kolitha.com/hcdt/sosa:Sensor
:sosa:Sensor rdf:type owl:Class ;
             rdfs:comment """Sensor - Device, agent (including humans), or software (simulation) involved in, or implementing, a Procedure. Sensors respond to a Stimulus, e.g., a change in the environment, or Input data composed from the Results of prior Observations, and generate a Result. Sensors can be hosted by Platforms.

https://www.w3.org/TR/vocab-ssn/#SOSASensor""" .


###  http://www.kolitha.com/hcdt/ssn-system:Latency
:ssn-system:Latency rdf:type owl:Class ;
                    rdfs:comment """Latency - The time between a command for an Observation (resp. Actuation) and the Sensor providing a Result (resp. the Actuator operating the Actuation), under the defined Conditions.

https://www.w3.org/TR/vocab-ssn/#SSNSYSTEMFrequency""" .


###  http://www.sws.org/sws/AIAcceptance
<http://www.sws.org/sws/AIAcceptance> rdf:type owl:Class ;
                                      rdfs:subClassOf <http://www.sws.org/sws/HumanCentricityFactor> .


###  http://www.sws.org/sws/Agency
<http://www.sws.org/sws/Agency> rdf:type owl:Class ;
                                rdfs:subClassOf <http://www.sws.org/sws/HumanCentricityFactor> .


###  http://www.sws.org/sws/EaseOfUse
<http://www.sws.org/sws/EaseOfUse> rdf:type owl:Class ;
                                   rdfs:subClassOf <http://www.sws.org/sws/HumanCentricityFactor> .


###  http://www.sws.org/sws/Ergonomics
<http://www.sws.org/sws/Ergonomics> rdf:type owl:Class ;
                                    rdfs:subClassOf <http://www.sws.org/sws/HumanCentricityFactor> .


###  http://www.sws.org/sws/Explainability
<http://www.sws.org/sws/Explainability> rdf:type owl:Class ;
                                        rdfs:subClassOf <http://www.sws.org/sws/HumanCentricityFactor> .


###  http://www.sws.org/sws/Fairness
<http://www.sws.org/sws/Fairness> rdf:type owl:Class ;
                                  rdfs:subClassOf <http://www.sws.org/sws/HumanCentricityFactor> .


###  http://www.sws.org/sws/FeedbackFromOthers
<http://www.sws.org/sws/FeedbackFromOthers> rdf:type owl:Class ;
                                            rdfs:subClassOf <http://www.sws.org/sws/HumanCentricityFactor> .


###  http://www.sws.org/sws/HumanCentricityFactor
<http://www.sws.org/sws/HumanCentricityFactor> rdf:type owl:Class ;
                                               rdfs:comment """A factor or condition that affects the experience, performance, or well-
being of human actors within the system""" .


###  http://www.sws.org/sws/Inclusivity
<http://www.sws.org/sws/Inclusivity> rdf:type owl:Class ;
                                     rdfs:subClassOf <http://www.sws.org/sws/HumanCentricityFactor> .


###  http://www.sws.org/sws/InformationProcessingNeeds
<http://www.sws.org/sws/InformationProcessingNeeds> rdf:type owl:Class ;
                                                    rdfs:subClassOf <http://www.sws.org/sws/HumanCentricityFactor> .


###  http://www.sws.org/sws/Interdependence
<http://www.sws.org/sws/Interdependence> rdf:type owl:Class ;
                                         rdfs:subClassOf <http://www.sws.org/sws/HumanCentricityFactor> .


###  http://www.sws.org/sws/Interpretability
<http://www.sws.org/sws/Interpretability> rdf:type owl:Class ;
                                          rdfs:subClassOf <http://www.sws.org/sws/HumanCentricityFactor> .


###  http://www.sws.org/sws/MentalDemands
<http://www.sws.org/sws/MentalDemands> rdf:type owl:Class ;
                                       rdfs:subClassOf <http://www.sws.org/sws/HumanCentricityFactor> .


###  http://www.sws.org/sws/PhysicalDemands
<http://www.sws.org/sws/PhysicalDemands> rdf:type owl:Class ;
                                         rdfs:subClassOf <http://www.sws.org/sws/HumanCentricityFactor> .


###  http://www.sws.org/sws/Privacy
<http://www.sws.org/sws/Privacy> rdf:type owl:Class ;
                                 rdfs:subClassOf <http://www.sws.org/sws/HumanCentricityFactor> .


###  http://www.sws.org/sws/ProblemSolving
<http://www.sws.org/sws/ProblemSolving> rdf:type owl:Class ;
                                        rdfs:subClassOf <http://www.sws.org/sws/HumanCentricityFactor> .


###  http://www.sws.org/sws/Satisfaction
<http://www.sws.org/sws/Satisfaction> rdf:type owl:Class ;
                                      rdfs:subClassOf <http://www.sws.org/sws/HumanCentricityFactor> .


###  http://www.sws.org/sws/SkillVariety
<http://www.sws.org/sws/SkillVariety> rdf:type owl:Class ;
                                      rdfs:subClassOf <http://www.sws.org/sws/HumanCentricityFactor> .


###  http://www.sws.org/sws/Stress
<http://www.sws.org/sws/Stress> rdf:type owl:Class ;
                                rdfs:subClassOf <http://www.sws.org/sws/HumanCentricityFactor> .


###  http://www.sws.org/sws/TaskVariety
<http://www.sws.org/sws/TaskVariety> rdf:type owl:Class ;
                                     rdfs:subClassOf <http://www.sws.org/sws/HumanCentricityFactor> .


###  http://www.sws.org/sws/WorkConditions
<http://www.sws.org/sws/WorkConditions> rdf:type owl:Class ;
                                        rdfs:subClassOf <http://www.sws.org/sws/HumanCentricityFactor> .


#################################################################
#    Individuals
#################################################################

###  http://www.kolitha.com/hcdt/AugmentedRealityInterface
:AugmentedRealityInterface rdf:type owl:NamedIndividual ,
                                    :Interface .


###  http://www.kolitha.com/hcdt/CommandLineInterface
:CommandLineInterface rdf:type owl:NamedIndividual ,
                               :Interface .


###  http://www.kolitha.com/hcdt/GraphicalUserInterface
:GraphicalUserInterface rdf:type owl:NamedIndividual ,
                                 :Interface .


###  http://www.kolitha.com/hcdt/VirtualRealityInterface
:VirtualRealityInterface rdf:type owl:NamedIndividual ,
                                  :Interface .


###  http://www.kolitha.com/hcdt/Worker1
:Worker1 rdf:type owl:NamedIndividual ,
                  :HumanActor ;
         :hasDigitalTwin :Worker1DT .


###  http://www.kolitha.com/hcdt/Worker1DT
:Worker1DT rdf:type owl:NamedIndividual ,
                    :HumanDigitalTwin .


[ <http://ontologydesignpatterns.org/opla-sd#entityPositionX> "349.5388954817158"^^xsd:double ;
  <http://ontologydesignpatterns.org/opla-sd#entityPositionY> "1020.0527261751465"^^xsd:double ;
  rdfs:comment "This is an entity positioning annotation generated by CoModIDE (https://comodide.com/). Removing this annotation will break rendering the CoModIDE schema diagram view."@en
] .

[ <http://ontologydesignpatterns.org/opla-sd#entityPositionX> "643.3562171180356"^^xsd:double ;
   <http://ontologydesignpatterns.org/opla-sd#entityPositionY> "131.64610522582066"^^xsd:double ;
   rdfs:comment "This is an entity positioning annotation generated by CoModIDE (https://comodide.com/). Removing this annotation will break rendering the CoModIDE schema diagram view."@en
 ] .

[ <http://ontologydesignpatterns.org/opla-sd#entityPositionX> "208.0051516249181"^^xsd:double ;
   <http://ontologydesignpatterns.org/opla-sd#entityPositionY> "291.3369547523279"^^xsd:double ;
   rdfs:comment "This is an entity positioning annotation generated by CoModIDE (https://comodide.com/). Removing this annotation will break rendering the CoModIDE schema diagram view."@en
 ] .

[ <http://ontologydesignpatterns.org/opla-sd#entityPositionX> "621.7504679876805"^^xsd:double ;
   <http://ontologydesignpatterns.org/opla-sd#entityPositionY> "222.5650647913749"^^xsd:double ;
   rdfs:comment "This is an entity positioning annotation generated by CoModIDE (https://comodide.com/). Removing this annotation will break rendering the CoModIDE schema diagram view."@en
 ] .

[ <http://ontologydesignpatterns.org/opla-sd#entityPositionX> "179.00418897878433"^^xsd:double ;
   <http://ontologydesignpatterns.org/opla-sd#entityPositionY> "221.04525642570886"^^xsd:double ;
   rdfs:comment "This is an entity positioning annotation generated by CoModIDE (https://comodide.com/). Removing this annotation will break rendering the CoModIDE schema diagram view."@en
 ] .

[ <http://ontologydesignpatterns.org/opla-sd#entityPositionX> "37.76644296556776"^^xsd:double ;
   <http://ontologydesignpatterns.org/opla-sd#entityPositionY> "159.5212246545486"^^xsd:double ;
   rdfs:comment "This is an entity positioning annotation generated by CoModIDE (https://comodide.com/). Removing this annotation will break rendering the CoModIDE schema diagram view."@en
 ] .

[ <http://ontologydesignpatterns.org/opla-sd#entityPositionX> "60.26013664051915"^^xsd:double ;
   <http://ontologydesignpatterns.org/opla-sd#entityPositionY> "730.1339929655369"^^xsd:double ;
   rdfs:comment "This is an entity positioning annotation generated by CoModIDE (https://comodide.com/). Removing this annotation will break rendering the CoModIDE schema diagram view."@en
 ] .

[ <http://ontologydesignpatterns.org/opla-sd#entityPositionX> "249.41970251485884"^^xsd:double ;
   <http://ontologydesignpatterns.org/opla-sd#entityPositionY> "690.1915665353059"^^xsd:double ;
   rdfs:comment "This is an entity positioning annotation generated by CoModIDE (https://comodide.com/). Removing this annotation will break rendering the CoModIDE schema diagram view."@en
 ] .

[ <http://ontologydesignpatterns.org/opla-sd#entityPositionX> "450.21530301176824"^^xsd:double ;
   <http://ontologydesignpatterns.org/opla-sd#entityPositionY> "859.8244131829491"^^xsd:double ;
   rdfs:comment "This is an entity positioning annotation generated by CoModIDE (https://comodide.com/). Removing this annotation will break rendering the CoModIDE schema diagram view."@en
 ] .

[ <http://ontologydesignpatterns.org/opla-sd#entityPositionX> "593.7411377469589"^^xsd:double ;
   <http://ontologydesignpatterns.org/opla-sd#entityPositionY> "169.94254147342315"^^xsd:double ;
   rdfs:comment "This is an entity positioning annotation generated by CoModIDE (https://comodide.com/). Removing this annotation will break rendering the CoModIDE schema diagram view."@en
 ] .

[ <http://ontologydesignpatterns.org/opla-sd#entityPositionX> "690.4497050807857"^^xsd:double ;
   <http://ontologydesignpatterns.org/opla-sd#entityPositionY> "690.1740263598009"^^xsd:double ;
   rdfs:comment "This is an entity positioning annotation generated by CoModIDE (https://comodide.com/). Removing this annotation will break rendering the CoModIDE schema diagram view."@en
 ] .

[ <http://ontologydesignpatterns.org/opla-sd#entityPositionX> "460.45787159805263"^^xsd:double ;
   <http://ontologydesignpatterns.org/opla-sd#entityPositionY> "610.4522380548324"^^xsd:double ;
   rdfs:comment "This is an entity positioning annotation generated by CoModIDE (https://comodide.com/). Removing this annotation will break rendering the CoModIDE schema diagram view."@en
 ] .

[ <http://ontologydesignpatterns.org/opla-sd#entityPositionX> "520.0149206197915"^^xsd:double ;
   <http://ontologydesignpatterns.org/opla-sd#entityPositionY> "990.3526570126105"^^xsd:double ;
   rdfs:comment "This is an entity positioning annotation generated by CoModIDE (https://comodide.com/). Removing this annotation will break rendering the CoModIDE schema diagram view."@en
 ] .

[ <http://ontologydesignpatterns.org/opla-sd#entityPositionX> "149.8528448213492"^^xsd:double ;
   <http://ontologydesignpatterns.org/opla-sd#entityPositionY> "959.5411488932568"^^xsd:double ;
   rdfs:comment "This is an entity positioning annotation generated by CoModIDE (https://comodide.com/). Removing this annotation will break rendering the CoModIDE schema diagram view."@en
 ] .

[ <http://ontologydesignpatterns.org/opla-sd#entityPositionX> "132.6653591775449"^^xsd:double ;
   <http://ontologydesignpatterns.org/opla-sd#entityPositionY> "269.8657549020317"^^xsd:double ;
   rdfs:comment "This is an entity positioning annotation generated by CoModIDE (https://comodide.com/). Removing this annotation will break rendering the CoModIDE schema diagram view."@en
 ] .

[ <http://ontologydesignpatterns.org/opla-sd#entityPositionX> "150.09350911560108"^^xsd:double ;
   <http://ontologydesignpatterns.org/opla-sd#entityPositionY> "1030.0432312318965"^^xsd:double ;
   rdfs:comment "This is an entity positioning annotation generated by CoModIDE (https://comodide.com/). Removing this annotation will break rendering the CoModIDE schema diagram view."@en
 ] .

[ <http://ontologydesignpatterns.org/opla-sd#entityPositionX> "227.20943688299707"^^xsd:double ;
   <http://ontologydesignpatterns.org/opla-sd#entityPositionY> "761.6320764227278"^^xsd:double ;
   rdfs:comment "This is an entity positioning annotation generated by CoModIDE (https://comodide.com/). Removing this annotation will break rendering the CoModIDE schema diagram view."@en
 ] .

[ <http://ontologydesignpatterns.org/opla-sd#entityPositionX> "640.4550244317408"^^xsd:double ;
   <http://ontologydesignpatterns.org/opla-sd#entityPositionY> "20.415746023646932"^^xsd:double ;
   rdfs:comment "This is an entity positioning annotation generated by CoModIDE (https://comodide.com/). Removing this annotation will break rendering the CoModIDE schema diagram view."@en
 ] .

[ <http://ontologydesignpatterns.org/opla-sd#entityPositionX> "585.1265310472049"^^xsd:double ;
   <http://ontologydesignpatterns.org/opla-sd#entityPositionY> "255.04531739751266"^^xsd:double ;
   rdfs:comment "This is an entity positioning annotation generated by CoModIDE (https://comodide.com/). Removing this annotation will break rendering the CoModIDE schema diagram view."@en
 ] .

[ <http://ontologydesignpatterns.org/opla-sd#entityPositionX> "124.70238066733776"^^xsd:double ;
   <http://ontologydesignpatterns.org/opla-sd#entityPositionY> "70.55835088724707"^^xsd:double ;
   rdfs:comment "This is an entity positioning annotation generated by CoModIDE (https://comodide.com/). Removing this annotation will break rendering the CoModIDE schema diagram view."@en
 ] .

[ <http://ontologydesignpatterns.org/opla-sd#entityPositionX> "186.28169920124836"^^xsd:double ;
   <http://ontologydesignpatterns.org/opla-sd#entityPositionY> "159.10126398906993"^^xsd:double ;
   rdfs:comment "This is an entity positioning annotation generated by CoModIDE (https://comodide.com/). Removing this annotation will break rendering the CoModIDE schema diagram view."@en
 ] .

[ <http://ontologydesignpatterns.org/opla-sd#entityPositionX> "118.51100689243451"^^xsd:double ;
   <http://ontologydesignpatterns.org/opla-sd#entityPositionY> "51.30189396152291"^^xsd:double ;
   rdfs:comment "This is an entity positioning annotation generated by CoModIDE (https://comodide.com/). Removing this annotation will break rendering the CoModIDE schema diagram view."@en
 ] .

[ <http://ontologydesignpatterns.org/opla-sd#entityPositionX> "659.6562606558017"^^xsd:double ;
   <http://ontologydesignpatterns.org/opla-sd#entityPositionY> "1000.2450238737072"^^xsd:double ;
   rdfs:comment "This is an entity positioning annotation generated by CoModIDE (https://comodide.com/). Removing this annotation will break rendering the CoModIDE schema diagram view."@en
 ] .

[ <http://ontologydesignpatterns.org/opla-sd#entityPositionX> "86.4831980795508"^^xsd:double ;
   <http://ontologydesignpatterns.org/opla-sd#entityPositionY> "17.72047206170261"^^xsd:double ;
   rdfs:comment "This is an entity positioning annotation generated by CoModIDE (https://comodide.com/). Removing this annotation will break rendering the CoModIDE schema diagram view."@en
 ] .

[ <http://ontologydesignpatterns.org/opla-sd#entityPositionX> "33.37112067776456"^^xsd:double ;
   <http://ontologydesignpatterns.org/opla-sd#entityPositionY> "94.05633169530623"^^xsd:double ;
   rdfs:comment "This is an entity positioning annotation generated by CoModIDE (https://comodide.com/). Removing this annotation will break rendering the CoModIDE schema diagram view."@en
 ] .

[ <http://ontologydesignpatterns.org/opla-sd#entityPositionX> "70.10691505870284"^^xsd:double ;
   <http://ontologydesignpatterns.org/opla-sd#entityPositionY> "839.7809771311606"^^xsd:double ;
   rdfs:comment "This is an entity positioning annotation generated by CoModIDE (https://comodide.com/). Removing this annotation will break rendering the CoModIDE schema diagram view."@en
 ] .

[ <http://ontologydesignpatterns.org/opla-sd#entityPositionX> "1.542547203063724"^^xsd:double ;
   <http://ontologydesignpatterns.org/opla-sd#entityPositionY> "119.14061112638026"^^xsd:double ;
   rdfs:comment "This is an entity positioning annotation generated by CoModIDE (https://comodide.com/). Removing this annotation will break rendering the CoModIDE schema diagram view."@en
 ] .

[ <http://ontologydesignpatterns.org/opla-sd#entityPositionX> "479.6979744014784"^^xsd:double ;
   <http://ontologydesignpatterns.org/opla-sd#entityPositionY> "615.5499507368929"^^xsd:double ;
   rdfs:comment "This is an entity positioning annotation generated by CoModIDE (https://comodide.com/). Removing this annotation will break rendering the CoModIDE schema diagram view."@en
 ] .

[ <http://ontologydesignpatterns.org/opla-sd#entityPositionX> "219.60397479155463"^^xsd:double ;
   <http://ontologydesignpatterns.org/opla-sd#entityPositionY> "738.6024586926977"^^xsd:double ;
   rdfs:comment "This is an entity positioning annotation generated by CoModIDE (https://comodide.com/). Removing this annotation will break rendering the CoModIDE schema diagram view."@en
 ] .

[ <http://ontologydesignpatterns.org/opla-sd#entityPositionX> "529.9693699063644"^^xsd:double ;
   <http://ontologydesignpatterns.org/opla-sd#entityPositionY> "839.8152290701676"^^xsd:double ;
   rdfs:comment "This is an entity positioning annotation generated by CoModIDE (https://comodide.com/). Removing this annotation will break rendering the CoModIDE schema diagram view."@en
 ] .

[ <http://ontologydesignpatterns.org/opla-sd#entityPositionX> "584.4117302794309"^^xsd:double ;
   <http://ontologydesignpatterns.org/opla-sd#entityPositionY> "125.25790258337997"^^xsd:double ;
   rdfs:comment "This is an entity positioning annotation generated by CoModIDE (https://comodide.com/). Removing this annotation will break rendering the CoModIDE schema diagram view."@en
 ] .

[ <http://ontologydesignpatterns.org/opla-sd#entityPositionX> "9.965722168401868"^^xsd:double ;
   <http://ontologydesignpatterns.org/opla-sd#entityPositionY> "569.6377147119933"^^xsd:double ;
   rdfs:comment "This is an entity positioning annotation generated by CoModIDE (https://comodide.com/). Removing this annotation will break rendering the CoModIDE schema diagram view."@en
 ] .

#################################################################
#    General axioms
#################################################################

[ rdf:type owl:AllDisjointClasses ;
   owl:members ( <http://www.sws.org/sws/AIAcceptance>
                 <http://www.sws.org/sws/Agency>
                 <http://www.sws.org/sws/EaseOfUse>
                 <http://www.sws.org/sws/Ergonomics>
                 <http://www.sws.org/sws/Explainability>
                 <http://www.sws.org/sws/Fairness>
                 <http://www.sws.org/sws/FeedbackFromOthers>
                 <http://www.sws.org/sws/Inclusivity>
                 <http://www.sws.org/sws/InformationProcessingNeeds>
                 <http://www.sws.org/sws/Interdependence>
                 <http://www.sws.org/sws/Interpretability>
                 <http://www.sws.org/sws/MentalDemands>
                 <http://www.sws.org/sws/PhysicalDemands>
                 <http://www.sws.org/sws/Privacy>
                 <http://www.sws.org/sws/ProblemSolving>
                 <http://www.sws.org/sws/Satisfaction>
                 <http://www.sws.org/sws/SkillVariety>
                 <http://www.sws.org/sws/Stress>
                 <http://www.sws.org/sws/TaskVariety>
                 <http://www.sws.org/sws/WorkConditions>
               )
 ] .


###  Generated by the OWL API (version 4.5.29.2024-05-13T12:11:03Z) https://github.com/owlcs/owlapi
