@prefix : <http://www.sws.org/sws#> .
@prefix owl: <http://www.w3.org/2002/07/owl#> .
@prefix rdf: <http://www.w3.org/1999/02/22-rdf-syntax-ns#> .
@prefix xml: <http://www.w3.org/XML/1998/namespace> .
@prefix xsd: <http://www.w3.org/2001/XMLSchema#> .
@prefix esco: <http://data.europa.eu/esco/model#> .
@prefix rdfs: <http://www.w3.org/2000/01/rdf-schema#> .
@prefix sosa: <http://www.w3.org/ns/sosa#> .
@base <http://www.sws.org/sws> .

<http://www.sws.org/sws> rdf:type owl:Ontology ;
                          owl:versionIRI <http://www.sws.org/sws/1.1.8> ;
                          rdfs:label "sws ontology" .

#################################################################
#    Annotation properties
#################################################################

###  http://www.w3.org/2000/01/rdf-schema#comment
rdfs:comment rdf:type owl:AnnotationProperty ;
             rdfs:label "comment" .


#################################################################
#    Datatypes
#################################################################

###  http://www.w3.org/1999/02/22-rdf-syntax-ns#langString
rdf:langString rdf:type rdfs:Datatype ;
               rdfs:label "langString" .


###  http://www.w3.org/2001/XMLSchema#double
xsd:double rdf:type rdfs:Datatype ;
           rdfs:label "double" .


###  http://www.w3.org/2001/XMLSchema#int
xsd:int rdf:type rdfs:Datatype ;
        rdfs:label "int" .


###  http://www.w3.org/2001/XMLSchema#integer
xsd:integer rdf:type rdfs:Datatype ;
            rdfs:label "integer" .


###  http://www.w3.org/2001/XMLSchema#string
xsd:string rdf:type rdfs:Datatype ;
           rdfs:label "string" .


###  http://www.w3.org/2002/07/owl#real
owl:real rdf:type rdfs:Datatype ;
         rdfs:label "real" .


#################################################################
#    Object Properties
#################################################################

###  http://www.sws.org/sws#actorHasPerformanceDimension
:actorHasPerformanceDimension rdf:type owl:ObjectProperty ;
                              rdfs:subPropertyOf :hasPerformanceDimension ;
                              rdfs:domain :Actor ;
                              rdfs:range :Performance ;
                              rdfs:label "actorHasPerformanceDimension" .


###  http://www.sws.org/sws#assignedTo
:assignedTo rdf:type owl:ObjectProperty ;
            rdfs:domain :Task ;
            rdfs:range :Actor ;
            rdfs:label "assignedTo" .


###  http://www.sws.org/sws#confidenceAssessmentHas
:confidenceAssessmentHas rdf:type owl:ObjectProperty ;
                         rdfs:label "confidenceAssessmentHas" .


###  http://www.sws.org/sws#confidenceAssessmentHasActor
:confidenceAssessmentHasActor rdf:type owl:ObjectProperty ;
                              rdfs:subPropertyOf :confidenceAssessmentHas ;
                              rdfs:domain :ConfidenceAssessment ;
                              rdfs:range :Actor ;
                              rdfs:label "confidenceAssessmentHasActor" .


###  http://www.sws.org/sws#confidenceAssessmentHasTask
:confidenceAssessmentHasTask rdf:type owl:ObjectProperty ;
                             rdfs:subPropertyOf :confidenceAssessmentHas ;
                             rdfs:domain :ConfidenceAssessment ;
                             rdfs:range :Task ;
                             rdfs:label "confidenceAssessmentHasTask" .


###  http://www.sws.org/sws#hasActorStatus
:hasActorStatus rdf:type owl:ObjectProperty ;
                rdfs:subPropertyOf :hasStatus ;
                rdfs:domain :Actor ;
                rdfs:range :ActorStatus ;
                rdfs:label "hasActorStatus" .


###  http://www.sws.org/sws#hasConstraint
:hasConstraint rdf:type owl:ObjectProperty ;
               rdfs:range :Constraint ;
               rdfs:label "hasConstraint" .


###  http://www.sws.org/sws#hasDecisionStatus
:hasDecisionStatus rdf:type owl:ObjectProperty ;
                   rdfs:subPropertyOf :hasStatus ;
                   rdfs:domain :Decision ;
                   rdfs:range :DecisionStatus ;
                   rdfs:label "hasDecisionStatus" .


###  http://www.sws.org/sws#hasDigitalTwin
:hasDigitalTwin rdf:type owl:ObjectProperty ;
                rdfs:domain :Actor ;
                rdfs:range :DigitalTwin ;
                rdfs:label "hasDigitalTwin" .


###  http://www.sws.org/sws#hasPerformanceDimension
:hasPerformanceDimension rdf:type owl:ObjectProperty ;
                         rdfs:range :Performance ;
                         rdfs:label "hasPerformanceDimension" .


###  http://www.sws.org/sws#hasSkill
:hasSkill rdf:type owl:ObjectProperty ;
          rdfs:domain :Actor ;
          rdfs:range esco:Skill ;
          rdfs:label "hasSkill" .


###  http://www.sws.org/sws#hasStatus
:hasStatus rdf:type owl:ObjectProperty ;
           rdfs:label "hasStatus" .


###  http://www.sws.org/sws#hasTask
:hasTask rdf:type owl:ObjectProperty ;
         rdfs:domain :Schedule ;
         rdfs:range :Task ;
         rdfs:label "hasTask" .


###  http://www.sws.org/sws#hasTaskStatus
:hasTaskStatus rdf:type owl:ObjectProperty ;
               rdfs:subPropertyOf :hasStatus ;
               rdfs:domain :Task ;
               rdfs:range :TaskStatus ;
               rdfs:label "hasTaskStatus" .


###  http://www.sws.org/sws#isAllocatedTo
:isAllocatedTo rdf:type owl:ObjectProperty ;
               rdfs:domain :Resource ;
               rdfs:range :Task ;
               rdfs:label "isAllocatedTo" .


###  http://www.sws.org/sws#isObservedBy
:isObservedBy rdf:type owl:ObjectProperty ;
              owl:inverseOf :observes ;
              rdfs:domain :NonHumanActor ;
              rdfs:range sosa:Sensor ;
              rdfs:label "isObservedBy" .


###  http://www.sws.org/sws#monitorsActor
:monitorsActor rdf:type owl:ObjectProperty ;
               rdfs:domain :DigitalTwin ;
               rdfs:range :Actor ;
               rdfs:label "monitorsActor" .


###  http://www.sws.org/sws#observes
:observes rdf:type owl:ObjectProperty ;
          rdfs:domain sosa:Sensor ;
          rdfs:range :NonHumanActor ;
          rdfs:label "observes" .


###  http://www.sws.org/sws#requiresResource
:requiresResource rdf:type owl:ObjectProperty ;
                  rdfs:domain :Task ;
                  rdfs:range :Resource ;
                  rdfs:label "requiresResource" .


###  http://www.sws.org/sws#requiresSkill
:requiresSkill rdf:type owl:ObjectProperty ;
               rdfs:domain :Task ;
               rdfs:range esco:Skill ;
               rdfs:label "requiresSkill" .


###  http://www.sws.org/sws#scheduleHasConstraint
:scheduleHasConstraint rdf:type owl:ObjectProperty ;
                       rdfs:subPropertyOf :hasConstraint ;
                       rdfs:domain :Schedule ;
                       rdfs:range :Constraint ;
                       rdfs:label "scheduleHasConstraint" .


###  http://www.sws.org/sws#scheduleHasPerformanceDimension
:scheduleHasPerformanceDimension rdf:type owl:ObjectProperty ;
                                 rdfs:subPropertyOf :hasPerformanceDimension ;
                                 rdfs:domain :Schedule ;
                                 rdfs:range :Performance ;
                                 rdfs:label "scheduleHasPerformanceDimension" .


###  http://www.sws.org/sws#taskHasConstraint
:taskHasConstraint rdf:type owl:ObjectProperty ;
                   rdfs:subPropertyOf :hasConstraint ;
                   rdfs:domain :Task ;
                   rdfs:range :Constraint ;
                   rdfs:label "taskHasConstraint" .


###  http://www.sws.org/sws#taskHasDecision
:taskHasDecision rdf:type owl:ObjectProperty ;
                 rdfs:domain :Task ;
                 rdfs:range :Decision ;
                 rdfs:label "taskHasDecision" .


###  http://www.sws.org/sws#taskHasPerformanceDimension
:taskHasPerformanceDimension rdf:type owl:ObjectProperty ;
                             rdfs:subPropertyOf :hasPerformanceDimension ;
                             rdfs:domain :Task ;
                             rdfs:range :Performance ;
                             rdfs:label "taskHasPerformanceDimension" .


###  http://www.sws.org/sws#triggersSliding
:triggersSliding rdf:type owl:ObjectProperty ;
                 rdfs:domain :Context ;
                 rdfs:range :Schedule ;
                 rdfs:label "triggersSliding" .


###  http://www.sws.org/sws#usesResource
:usesResource rdf:type owl:ObjectProperty ;
              rdfs:domain :Actor ;
              rdfs:range :Resource ;
              rdfs:label "usesResource" .


#################################################################
#    Data properties
#################################################################

###  http://www.sws.org/sws#hasActorRole
:hasActorRole rdf:type owl:DatatypeProperty ;
              rdfs:domain :Actor ;
              rdfs:range xsd:string ;
              rdfs:label "hasActorRole" .


###  http://www.sws.org/sws#hasActorStatusDescriptor
:hasActorStatusDescriptor rdf:type owl:DatatypeProperty ;
                          rdfs:domain :ActorStatus ;
                          rdfs:range xsd:string ;
                          rdfs:label "hasActorStatusDescriptor" .


###  http://www.sws.org/sws#hasConfidence
:hasConfidence rdf:type owl:DatatypeProperty ;
               rdfs:domain :ConfidenceAssessment ;
               rdfs:range xsd:decimal ;
               rdfs:label "hasConfidence" .


###  http://www.sws.org/sws#hasDecisionStatusDescriptor
:hasDecisionStatusDescriptor rdf:type owl:DatatypeProperty ;
                             rdfs:domain :DecisionStatus ;
                             rdfs:range xsd:string ;
                             rdfs:label "hasDecisionStatusDescriptor" .


###  http://www.sws.org/sws#hasOperationalPerformanceScore
:hasOperationalPerformanceScore rdf:type owl:DatatypeProperty ;
                                rdfs:subPropertyOf :hasPerformanceScore ;
                                rdfs:domain :Operational ;
                                rdfs:range xsd:decimal ;
                                rdfs:label "hasOperationalPerformanceScore" .


###  http://www.sws.org/sws#hasPerformanceScore
:hasPerformanceScore rdf:type owl:DatatypeProperty ;
                     rdfs:domain :Performance ;
                     rdfs:range xsd:decimal ;
                     rdfs:label "hasPerformanceScore" .


###  http://www.sws.org/sws#hasPriorityLevel
:hasPriorityLevel rdf:type owl:DatatypeProperty ;
                  rdfs:domain :Task ;
                  rdfs:range xsd:int ;
                  rdfs:label "hasPriorityLevel" .


###  http://www.sws.org/sws#hasSensorValue
:hasSensorValue rdf:type owl:DatatypeProperty ;
                rdfs:domain sosa:Sensor ;
                rdfs:range owl:real ;
                rdfs:label "hasSensorValue" .


###  http://www.sws.org/sws#hasSkillLevel
:hasSkillLevel rdf:type owl:DatatypeProperty ;
               rdfs:domain :Actor ;
               rdfs:range xsd:integer ;
               rdfs:label "hasSkillLevel" .


###  http://www.sws.org/sws#hasSocialPerformanceScore
:hasSocialPerformanceScore rdf:type owl:DatatypeProperty ;
                           rdfs:subPropertyOf :hasPerformanceScore ;
                           rdfs:domain :Social ;
                           rdfs:range xsd:decimal ;
                           rdfs:label "hasSocialPerformanceScore" .


###  http://www.sws.org/sws#hasTaskComplexity
:hasTaskComplexity rdf:type owl:DatatypeProperty ;
                   rdfs:domain :Task ;
                   rdfs:range xsd:string ;
                   rdfs:label "hasTaskComplexity" .


###  http://www.sws.org/sws#hasTaskStatusDescriptor
:hasTaskStatusDescriptor rdf:type owl:DatatypeProperty ;
                         rdfs:domain :TaskStatus ;
                         rdfs:range xsd:string ;
                         rdfs:label "hasTaskStatusDescriptor" .


###  http://www.sws.org/sws#hasTechnicalPerformanceScore
:hasTechnicalPerformanceScore rdf:type owl:DatatypeProperty ;
                              rdfs:subPropertyOf :hasPerformanceScore ;
                              rdfs:domain :Technical ;
                              rdfs:range xsd:decimal ;
                              rdfs:label "hasTechnicalPerformanceScore" .


#################################################################
#    Classes
#################################################################

###  http://data.europa.eu/esco/model#Skill
esco:Skill rdf:type owl:Class ;
           rdfs:comment "A capability or competence possessed by an actor, based on the ESCO taxonomy." ;
           rdfs:label "Skill" .


###  http://www.sws.org/sws#AIAcceptance
:AIAcceptance rdf:type owl:Class ;
              rdfs:subClassOf :Social ;
              rdfs:comment "AI acceptance measurements quantify the degree to which human actors (usually workers) accept the AI agents’ presence in a work environment." ;
              rdfs:label "AIAcceptance" .


###  http://www.sws.org/sws#Accuracy
:Accuracy rdf:type owl:Class ;
          rdfs:subClassOf :Technical ;
          rdfs:comment "Accuracy meatrics measure the degree to which an AI model generates a correct output for the problem given the available data." ;
          rdfs:label "Accuracy" .


###  http://www.sws.org/sws#Actor
:Actor rdf:type owl:Class ;
       rdfs:comment "Represents an entity capable of performing tasks or making decisions." ;
       rdfs:label "Actor" .


###  http://www.sws.org/sws#ActorStatus
:ActorStatus rdf:type owl:Class ;
             rdfs:subClassOf :Status ;
             rdfs:label "ActorStatus" .


###  http://www.sws.org/sws#Agency
:Agency rdf:type owl:Class ;
        rdfs:subClassOf :Social ;
        rdfs:comment "Agency metrics traditionally measure the discretion of human agents when making decisions to carry out work (human agency)." ;
        rdfs:label "Agency" .


###  http://www.sws.org/sws#ConfidenceAssessment
:ConfidenceAssessment rdf:type owl:Class ;
                      rdfs:label "ConfidenceAssessment" .


###  http://www.sws.org/sws#Constraint
:Constraint rdf:type owl:Class ;
            rdfs:comment "Defines any limitation, requirement, or boundary condition that affects task execution and must not be violated by a schedule." ;
            rdfs:label "Constraint" .


###  http://www.sws.org/sws#Context
:Context rdf:type owl:Class ;
         rdfs:comment "Any information that can be used to characterize the situation of an entity." ;
         rdfs:label "Context" .


###  http://www.sws.org/sws#ContinuantResource
:ContinuantResource rdf:type owl:Class ;
                    rdfs:subClassOf :Resource ;
                    owl:disjointWith :OccurrentResource ;
                    rdfs:comment "Resources that continue to persist through time while maintaining their identity. (IFO/BFO)" ;
                    rdfs:label "ContinuantResource" .


###  http://www.sws.org/sws#CostBenefitRatios
:CostBenefitRatios rdf:type owl:Class ;
                   rdfs:subClassOf :Operational ;
                   rdfs:comment "The cost/benefit ratios are measures associating the costs relative to the benefits of a process and are indicative of the potential profit margins of operations." ;
                   rdfs:label "CostBenefitRatios" .


###  http://www.sws.org/sws#Costs
:Costs rdf:type owl:Class ;
       rdfs:subClassOf :Operational ;
       rdfs:comment "Cost metrics measure the costs associated with a process." ;
       rdfs:label "Costs" .


###  http://www.sws.org/sws#CycleTime
:CycleTime rdf:type owl:Class ;
           rdfs:subClassOf :Operational ;
           rdfs:comment "Cycle time indicators measure the elapsed time between initiating and completing a task, process, or machine operation." ;
           rdfs:label "CycleTime" .


###  http://www.sws.org/sws#Decision
:Decision rdf:type owl:Class ;
          rdfs:comment "Representing the conclusion or choice among alternatives to allocate tasks, adjust schedules, or adaptive strategies" ;
          rdfs:label "Decision" .


###  http://www.sws.org/sws#DecisionStatus
:DecisionStatus rdf:type owl:Class ;
                rdfs:subClassOf :Status ;
                rdfs:label "DecisionStatus" .


###  http://www.sws.org/sws#DeliveryReliability
:DeliveryReliability rdf:type owl:Class ;
                     rdfs:subClassOf :Operational ;
                     rdfs:comment "Delivery reliability metrics measure a supplier’s capacity to serve customers on time." ;
                     rdfs:label "DeliveryReliability" .


###  http://www.sws.org/sws#DependentContinuants
:DependentContinuants rdf:type owl:Class ;
                      rdfs:subClassOf :ContinuantResource ;
                      rdfs:comment "cannot exist without an independent continuant. (qualities of a product)" ;
                      rdfs:label "DependentContinuants" .


###  http://www.sws.org/sws#DeploymentCosts
:DeploymentCosts rdf:type owl:Class ;
                 rdfs:subClassOf :Operational ;
                 rdfs:comment "Indicators measuring the cost of deploying a solution in an operational environment." ;
                 rdfs:label "DeploymentCosts" .


###  http://www.sws.org/sws#DerivedContext
:DerivedContext rdf:type owl:Class ;
                rdfs:subClassOf :Context ;
                rdfs:comment "Context inferred from raw data or calculated through processing, reasoning, or interpretations. (e.g., Workload)" ;
                rdfs:label "DerivedContext" .


###  http://www.sws.org/sws#DigitalTwin
:DigitalTwin rdf:type owl:Class ;
             rdfs:comment "The real-time digital representation of a physical actor, environment, or process." ;
             rdfs:label "DigitalTwin" .


###  http://www.sws.org/sws#DigitalTwinDecision
:DigitalTwinDecision rdf:type owl:Class ;
                     rdfs:subClassOf :Decision ;
                     rdfs:comment "A decision made by DigitalTwin" ;
                     rdfs:label "DigitalTwinDecision" .


###  http://www.sws.org/sws#EaseOfUse
:EaseOfUse rdf:type owl:Class ;
           rdfs:subClassOf :Social ;
           rdfs:comment "Ease of use metrics measure the accessibility of a system’s functionalities to a user and the ease of learning to use the system effectively and efficiently." ;
           rdfs:label "EaseOfUse" .


###  http://www.sws.org/sws#EnvironmentalSustainability
:EnvironmentalSustainability rdf:type owl:Class ;
                             rdfs:subClassOf :Operational ;
                             rdfs:comment "Environmental sustainability metrics measure the environmental impact of a process." ;
                             rdfs:label "EnvironmentalSustainability" .


###  http://www.sws.org/sws#Explainability
:Explainability rdf:type owl:Class ;
                rdfs:subClassOf :Social ;
                rdfs:comment "Explainability refers to the capacity of a system to provide humans with comprehensible explanations of its decisions and the rationale of its actions (outcome-centric understandability)." ;
                rdfs:label "Explainability" .


###  http://www.sws.org/sws#Fairness
:Fairness rdf:type owl:Class ;
          rdfs:subClassOf :Social ;
          rdfs:comment "Fairness assessments quantify a system’s non-discrimination capabilities." ;
          rdfs:label "Fairness" .


###  http://www.sws.org/sws#FeedbackFromOthers
:FeedbackFromOthers rdf:type owl:Class ;
                    rdfs:subClassOf :Social ;
                    rdfs:comment "Feedback metrics measure the degree of feedback provided to a worker in a work environment." ;
                    rdfs:label "FeedbackFromOthers" .


###  http://www.sws.org/sws#Flexibility
:Flexibility rdf:type owl:Class ;
             rdfs:subClassOf :Operational ;
             rdfs:comment "Flexibility measures capture the degree to which processes can be modified to address changes in operational requirements." ;
             rdfs:label "Flexibility" .


###  http://www.sws.org/sws#HardConstraint
:HardConstraint rdf:type owl:Class ;
                rdfs:subClassOf :Constraint ;
                rdfs:comment "A non-negotiable constraint that must always be satisfied by any schedule" ;
                rdfs:label "HardConstraint" .


###  http://www.sws.org/sws#HumanActor
:HumanActor rdf:type owl:Class ;
            rdfs:subClassOf :Actor ;
            owl:disjointWith :NonHumanActor ;
            rdfs:comment "A subclass of Actor representing a human entity involved in performing tasks or making decisions" ;
            rdfs:label "HumanActor" .


###  http://www.sws.org/sws#HumanDecision
:HumanDecision rdf:type owl:Class ;
               rdfs:subClassOf :Decision ;
               rdfs:comment "A decision made solely by a human actor" ;
               rdfs:label "HumanDecision" .


###  http://www.sws.org/sws#Inclusivity
:Inclusivity rdf:type owl:Class ;
             rdfs:subClassOf :Social ;
             rdfs:comment "Inclusivity indicators quantify the practice of providing equal access to opportunities and resources for users, especially users belonging to minority groups or traditionally misrepresented groups." ;
             rdfs:label "Inclusivity" .


###  http://www.sws.org/sws#IndependentContinuants
:IndependentContinuants rdf:type owl:Class ;
                        rdfs:subClassOf :ContinuantResource ;
                        rdfs:comment "Do not depend on other resources for their existence. (e.g., person, machine, product)" ;
                        rdfs:label "IndependentContinuants" .


###  http://www.sws.org/sws#InformationProcessingNeeds
:InformationProcessingNeeds rdf:type owl:Class ;
                            rdfs:subClassOf :Social ;
                            rdfs:comment "Information processing measures quantify the requirements of interpreting, gathering, and synthesising information for decision-making purposes." ;
                            rdfs:label "InformationProcessingNeeds" .


###  http://www.sws.org/sws#Interdependence
:Interdependence rdf:type owl:Class ;
                 rdfs:subClassOf :Social ;
                 rdfs:comment "Interdependence indicators measure the degree to which a process' (human) actors depend on each other." ;
                 rdfs:label "Interdependence" .


###  http://www.sws.org/sws#Interpretability
:Interpretability rdf:type owl:Class ;
                  rdfs:subClassOf :Social ;
                  rdfs:comment "Interpretability metrics measure the ability to translate a system’s working principles into human-understandable language (model design-centric understandability)." ;
                  rdfs:label "Interpretability" .


###  http://www.sws.org/sws#JointDecision
:JointDecision rdf:type owl:Class ;
               rdfs:subClassOf :Decision ;
               rdfs:comment "A decision made through collaboration between human and non-human actors" ;
               rdfs:label "JointDecision" .


###  http://www.sws.org/sws#Latency
:Latency rdf:type owl:Class ;
         rdfs:subClassOf :Technical ;
         rdfs:comment "Latency measures a system’s responsiveness, typically in terms of the time it takes to process one unit of data." ;
         rdfs:label "Latency" .


###  http://www.sws.org/sws#MentalDemands
:MentalDemands rdf:type owl:Class ;
               rdfs:subClassOf :Social ;
               rdfs:comment "Mental demands measurements quantify the cognitive costs associated with performing a task." ;
               rdfs:label "MentalDemands" .


###  http://www.sws.org/sws#NonDerivedContext
:NonDerivedContext rdf:type owl:Class ;
                   rdfs:subClassOf :Context ;
                   rdfs:comment "Raw or directly observable contextual information (e.g., Temperature, Heart Rate)" ;
                   rdfs:label "NonDerivedContext" .


###  http://www.sws.org/sws#NonHumanActor
:NonHumanActor rdf:type owl:Class ;
               rdfs:subClassOf :Actor ;
               rdfs:comment "A subclass of Actor representing artificial or automated entities, such as robots, AI or software, capable of performing tasks or making decisions." ;
               rdfs:label "NonHumanActor" .


###  http://www.sws.org/sws#OccurrentResource
:OccurrentResource rdf:type owl:Class ;
                   rdfs:subClassOf :Resource ;
                   rdfs:comment """Resources occur, happen or unfold in time. (IFO/BFO)

Occurrents can be entities that
1. are a part of time, such as a time instant or time period
2. exist in time by occurring or happening such as a manufacturing process
3. represent a boundary of an occurrence or happening such as the beginning of a process.

ref:The Industrial Ontologies Foundry (IOF) Core Ontology""" ;
                   rdfs:label "OccurrentResource" .


###  http://www.sws.org/sws#Operational
:Operational rdf:type owl:Class ;
             rdfs:subClassOf :Performance ;
             rdfs:comment "Operational evaluation metrics are used to measure the economic performance of operational units." ;
             rdfs:label "Operational" .


###  http://www.sws.org/sws#PerceivedQuality
:PerceivedQuality rdf:type owl:Class ;
                  rdfs:subClassOf :Operational ;
                  rdfs:comment "Perceived quality metrics measure the perceived satisfaction with a process’ output." ;
                  rdfs:label "PerceivedQuality" .


###  http://www.sws.org/sws#Performance
:Performance rdf:type owl:Class ;
             rdfs:label "Performance" .


###  http://www.sws.org/sws#PhysicalDemands
:PhysicalDemands rdf:type owl:Class ;
                 rdfs:subClassOf :Social ;
                 rdfs:comment "Physical demands measurements quantify the physical efforts associated with performing a work task." ;
                 rdfs:label "PhysicalDemands" .


###  http://www.sws.org/sws#PhysicalErgonomics
:PhysicalErgonomics rdf:type owl:Class ;
                    rdfs:subClassOf :Social ;
                    rdfs:comment "Physical ergonomics indicators reflect how a task or process allows workers to maintain correct postures and proper movements." ;
                    rdfs:label "PhysicalErgonomics" .


###  http://www.sws.org/sws#Privacy
:Privacy rdf:type owl:Class ;
         rdfs:subClassOf :Social ;
         rdfs:comment "Privacy indicators measure a system’s capacity to ensure informational privacy." ;
         rdfs:label "Privacy" .


###  http://www.sws.org/sws#ProblemSolving
:ProblemSolving rdf:type owl:Class ;
                rdfs:subClassOf :Social ;
                rdfs:comment "Problem-solving indicators assess the degree of innovativeness required for completing a task." ;
                rdfs:label "ProblemSolving" .


###  http://www.sws.org/sws#Productivity
:Productivity rdf:type owl:Class ;
              rdfs:subClassOf :Operational ;
              rdfs:comment "Productivity metrics measure the efficiency of a production process." ;
              rdfs:label "Productivity" .


###  http://www.sws.org/sws#Quality
:Quality rdf:type owl:Class ;
         rdfs:subClassOf :Operational ;
         rdfs:comment "Quality metrics measure the degree to which a process meets the demanded specifications or requirements." ;
         rdfs:label "Quality" .


###  http://www.sws.org/sws#Reliability
:Reliability rdf:type owl:Class ;
             rdfs:subClassOf :Technical ;
             rdfs:comment "Reliability metrics evaluate whether the AI system behaves according to its design intentions." ;
             rdfs:label "Reliability" .


###  http://www.sws.org/sws#Resource
:Resource rdf:type owl:Class ;
          rdfs:label "Resource" .


###  http://www.sws.org/sws#ReturnOnInvestment
:ReturnOnInvestment rdf:type owl:Class ;
                    rdfs:subClassOf :Operational ;
                    rdfs:comment "Return on investment is an investment’s profitability measure." ;
                    rdfs:label "ReturnOnInvestment" .


###  http://www.sws.org/sws#Robustness
:Robustness rdf:type owl:Class ;
            rdfs:subClassOf :Technical ;
            rdfs:comment "Robustness measures the ability of an AI system to perform in varying circumstances, e.g., in variations in the input data and context." ;
            rdfs:label "Robustness" .


###  http://www.sws.org/sws#RoutingFlexibility
:RoutingFlexibility rdf:type owl:Class ;
                    rdfs:subClassOf :Operational ;
                    rdfs:comment "Routing flexibility measures assess the capability of a process to complete an operation in multiple ways." ;
                    rdfs:label "RoutingFlexibility" .


###  http://www.sws.org/sws#Safety
:Safety rdf:type owl:Class ;
        rdfs:subClassOf :Technical ;
        rdfs:comment "Safety refers to a system’s capability to minimise unintentional harm stemming either from unexpected system actions or misuse of human operators." ;
        rdfs:label "Safety" .


###  http://www.sws.org/sws#Satisfaction
:Satisfaction rdf:type owl:Class ;
              rdfs:subClassOf :Social ;
              rdfs:comment "Satisfaction metrics measure an operator’s contentment with a process’ performance." ;
              rdfs:label "Satisfaction" .


###  http://www.sws.org/sws#Scalability
:Scalability rdf:type owl:Class ;
             rdfs:subClassOf :Technical ;
             rdfs:comment "Scalability concerns a system’s ability to maintain its operational capacities in response to changes (typically up-scaling) of processing and input data demands." ;
             rdfs:label "Scalability" .


###  http://www.sws.org/sws#Schedule
:Schedule rdf:type owl:Class ;
          rdfs:label "Schedule" .


###  http://www.sws.org/sws#Security
:Security rdf:type owl:Class ;
          rdfs:subClassOf :Technical ;
          rdfs:comment "Security refers to a system’s ability to prevent unintended execution, unauthorised access, and data leakage." ;
          rdfs:label "Security" .


###  http://www.sws.org/sws#SkillVariety
:SkillVariety rdf:type owl:Class ;
              rdfs:subClassOf :Social ;
              rdfs:comment "Skill variety metrics measure the range of skills needed for a task or process." ;
              rdfs:label "SkillVariety" .


###  http://www.sws.org/sws#Social
:Social rdf:type owl:Class ;
        rdfs:subClassOf :Performance ;
        rdfs:comment "Social indicators measure qualitative and quantitative aspects of work design from a human involvement perspective." ;
        rdfs:label "Social" .


###  http://www.sws.org/sws#SoftConstraint
:SoftConstraint rdf:type owl:Class ;
                rdfs:subClassOf :Constraint ;
                rdfs:comment "A preferred constraint that may be relaxed if necessary to accommodate a schedule" ;
                rdfs:label "SoftConstraint" .


###  http://www.sws.org/sws#Status
:Status rdf:type owl:Class ;
        rdfs:label "Status" .


###  http://www.sws.org/sws#Stress
:Stress rdf:type owl:Class ;
        rdfs:subClassOf :Social ;
        rdfs:comment "Stress indicators measure the degree of mental or emotional strain resulting from demanding work circumstances." ;
        rdfs:label "Stress" .


###  http://www.sws.org/sws#Task
:Task rdf:type owl:Class ;
      rdfs:label "Task" .


###  http://www.sws.org/sws#TaskStatus
:TaskStatus rdf:type owl:Class ;
            rdfs:subClassOf :Status ;
            rdfs:label "TaskStatus" .


###  http://www.sws.org/sws#TaskVariety
:TaskVariety rdf:type owl:Class ;
             rdfs:subClassOf :Social ;
             rdfs:comment "Task variety metrics quantify the variability and range of performed tasks." ;
             rdfs:label "TaskVariety" .


###  http://www.sws.org/sws#Technical
:Technical rdf:type owl:Class ;
           rdfs:subClassOf :Performance ;
           rdfs:comment "Technical evaluation metrics are used to assess the performance of AI components in terms of their technical capabilities." ;
           rdfs:label "Technical" .


###  http://www.sws.org/sws#WorkConditions
:WorkConditions rdf:type owl:Class ;
                rdfs:subClassOf :Social ;
                rdfs:comment "Work condition metrics assess the appropriateness and appeal of the environment where a task is performed." ;
                rdfs:label "WorkConditions" .


###  http://www.w3.org/ns/sosa#Sensor
sosa:Sensor rdf:type owl:Class ;
            rdfs:comment """Sensors respond to a Stimulus, e.g., a change in the environment, or Input data composed from the Results of prior Observations, and generate a Result.

https://www.w3.org/TR/vocab-ssn/#SOSASensor""" ;
            rdfs:label "Sensor" .


#################################################################
#    Individuals
#################################################################

###  http://www.sws.org/sws#AcceptDecision
:AcceptDecision rdf:type owl:NamedIndividual ,
                         :DecisionStatus ;
                rdfs:label "AcceptDecision" .


###  http://www.sws.org/sws#ActorAvailable
:ActorAvailable rdf:type owl:NamedIndividual ,
                         :ActorStatus ;
                rdfs:label "ActorAvailable" .


###  http://www.sws.org/sws#ActorBusy
:ActorBusy rdf:type owl:NamedIndividual ,
                    :ActorStatus ;
           rdfs:label "ActorBusy" .


###  http://www.sws.org/sws#ActorUnavailable
:ActorUnavailable rdf:type owl:NamedIndividual ,
                           :ActorStatus ;
                  rdfs:label "ActorUnavailable" .


###  http://www.sws.org/sws#AdmissibleSchedule
:AdmissibleSchedule rdf:type owl:NamedIndividual ,
                             :Schedule ;
                    rdfs:label "AdmissibleSchedule" .


###  http://www.sws.org/sws#MasterSchedule
:MasterSchedule rdf:type owl:NamedIndividual ,
                         :Schedule ;
                rdfs:label "MasterSchedule" .


###  http://www.sws.org/sws#RejectDecision
:RejectDecision rdf:type owl:NamedIndividual ,
                         :DecisionStatus ;
                rdfs:label "RejectDecision" .


###  http://www.sws.org/sws#TaskCompleted
:TaskCompleted rdf:type owl:NamedIndividual ,
                        :TaskStatus ;
               rdfs:label "TaskCompleted" .


###  http://www.sws.org/sws#TaskInProgress
:TaskInProgress rdf:type owl:NamedIndividual ,
                         :TaskStatus ;
                rdfs:label "TaskInProgress" .


###  http://www.sws.org/sws#TaskPending
:TaskPending rdf:type owl:NamedIndividual ,
                      :TaskStatus ;
             rdfs:label "TaskPending" .


#################################################################
#    General axioms
#################################################################

[ rdf:type owl:AllDisjointClasses ;
  owl:members ( esco:Skill
                :Actor
                :ConfidenceAssessment
                :Constraint
                :Context
                :Decision
                :DigitalTwin
                :Performance
                :Resource
                :Schedule
                :Status
                :Task
                sosa:Sensor
              )
] .


###  Generated by the OWL API (version 4.5.26) https://github.com/owlcs/owlapi
